Finishing Module Globals. It however requires far too much memory for compilation.

low/Globals.v
@@ -9,29 +9,71 @@ Require Export RinternalsAux.
 (** Global variables that are initialised once, then treated as
   constants.  They are initialised in the file Rinit.v. **)
 Record Globals := make_Globals {
-    R_NilValue : SExpRec_pointer ;
-
-    R_EmptyEnv : SExpRec_pointer ;
+    R_AsCharacterSymbol : SExpRec_pointer ;
     R_BaseEnv : SExpRec_pointer ;
-    R_GlobalEnv : SExpRec_pointer ;
-    R_BaseNamespace : SExpRec_pointer ;
     R_BaseNamespaceName : SExpRec_pointer ;
+    R_BaseNamespace : SExpRec_pointer ;
     R_BaseSymbol : SExpRec_pointer ;
+    R_BraceSymbol : SExpRec_pointer ;
+    R_Bracket2Symbol : SExpRec_pointer ;
+    R_BracketSymbol : SExpRec_pointer ;
+    R_ClassSymbol : SExpRec_pointer ;
+    R_ColonSymbol : SExpRec_pointer ;
+    R_CommentSymbol : SExpRec_pointer ;
+    R_ConnIdSymbol : SExpRec_pointer ;
+    R_DevicesSymbol : SExpRec_pointer ;
+    R_DeviceSymbol : SExpRec_pointer ;
+    R_DimNamesSymbol : SExpRec_pointer ;
+    R_DimSymbol : SExpRec_pointer ;
+    R_DollarSymbol : SExpRec_pointer ;
+    R_dot_Class : SExpRec_pointer ;
+    R_dot_defined : SExpRec_pointer ;
+    R_DotEnvSymbol : SExpRec_pointer ;
+    R_dot_GenericCallEnv : SExpRec_pointer ;
+    R_dot_GenericDefEnv : SExpRec_pointer ;
+    R_dot_Generic : SExpRec_pointer ;
+    R_dot_Group : SExpRec_pointer ;
+    R_dot_Method : SExpRec_pointer ;
+    R_dot_Methods : SExpRec_pointer ;
+    R_dot_packageName : SExpRec_pointer ;
+    R_DotsSymbol : SExpRec_pointer ;
+    R_dot_target : SExpRec_pointer ;
+    R_DoubleColonSymbol : SExpRec_pointer ;
+    R_DropSymbol : SExpRec_pointer ;
+    R_EmptyEnv : SExpRec_pointer ;
+    R_ExactSymbol : SExpRec_pointer ;
+    R_FalseValue : SExpRec_pointer ;
+    R_GlobalEnv : SExpRec_pointer ;
+    R_LevelsSymbol : SExpRec_pointer ;
+    R_LogicalNAValue : SExpRec_pointer ;
+    R_MethodsNamespace : SExpRec_pointer ;
+    R_MissingArg : SExpRec_pointer ;
+    R_ModeSymbol : SExpRec_pointer ;
+    R_NamespaceEnvSymbol : SExpRec_pointer ;
     R_NamespaceRegistry : SExpRec_pointer ;
     R_NamespaceSymbol : SExpRec_pointer ;
-    R_MethodsNamespace : SExpRec_pointer ;
-
-    R_TrueValue : SExpRec_pointer ;
-    R_FalseValue : SExpRec_pointer ;
-    R_LogicalNAValue : SExpRec_pointer ;
-
-    R_UnboundValue : SExpRec_pointer ;
-    R_MissingArg : SExpRec_pointer ;
-    R_DotsSymbol : SExpRec_pointer ;
+    R_NamesSymbol : SExpRec_pointer ;
+    R_NameSymbol  : SExpRec_pointer ;
+    R_NaRmSymbol : SExpRec_pointer ;
+    R_NilValue : SExpRec_pointer ;
+    R_PackageSymbol : SExpRec_pointer ;
+    R_PreviousSymbol : SExpRec_pointer ;
     R_QuoteSymbol : SExpRec_pointer ;
-
-    R_ClassSymbol : SExpRec_pointer ;
-    R_RowNamesSymbol : SExpRec_pointer
+    R_RecursiveSymbol : SExpRec_pointer ;
+    R_RowNamesSymbol : SExpRec_pointer ;
+    R_SeedsSymbol : SExpRec_pointer ;
+    R_SortListSymbol : SExpRec_pointer ;
+    R_SourceSymbol : SExpRec_pointer ;
+    R_SpecSymbol : SExpRec_pointer ;
+    R_SrcfileSymbol : SExpRec_pointer ;
+    R_SrcrefSymbol : SExpRec_pointer ;
+    R_TmpvalSymbol : SExpRec_pointer ;
+    R_TripleColonSymbol : SExpRec_pointer ;
+    R_TrueValue : SExpRec_pointer ;
+    R_TspSymbol : SExpRec_pointer ;
+    R_UnboundValue : SExpRec_pointer ;
+    R_UseNamesSymbol : SExpRec_pointer ;
+    R_WholeSrcrefSymbol : SExpRec_pointer ;
   }.
 
 
@@ -40,157 +82,77 @@ Record Globals := make_Globals {
  * in Coq. As we are going to need it (as it helps avoid mistakes in
  * this particular case), we implement a specialised version in Ltac. **)
 
-(** Here follows a list of all the constructors of [Globals]. **)
-Definition Globals_constructors :=
-  [ R_NilValue ;
-    R_EmptyEnv ;
+(** Here follows a list of all the projections of [Globals]. **)
+Definition Globals_projections :=
+  [ R_AsCharacterSymbol ;
     R_BaseEnv ;
-    R_GlobalEnv ;
-    R_BaseNamespace ;
     R_BaseNamespaceName ;
+    R_BaseNamespace ;
     R_BaseSymbol ;
+    R_BraceSymbol ;
+    R_Bracket2Symbol ;
+    R_BracketSymbol ;
+    R_ClassSymbol ;
+    R_ColonSymbol ;
+    R_CommentSymbol ;
+    R_ConnIdSymbol ;
+    R_DevicesSymbol ;
+    R_DeviceSymbol ;
+    R_DimNamesSymbol ;
+    R_DimSymbol ;
+    R_DollarSymbol ;
+    R_dot_Class ;
+    R_dot_defined ;
+    R_DotEnvSymbol ;
+    R_dot_GenericCallEnv ;
+    R_dot_GenericDefEnv ;
+    R_dot_Generic ;
+    R_dot_Group ;
+    R_dot_Method ;
+    R_dot_Methods ;
+    R_dot_packageName ;
+    R_DotsSymbol ;
+    R_dot_target ;
+    R_DoubleColonSymbol ;
+    R_DropSymbol ;
+    R_EmptyEnv ;
+    R_ExactSymbol ;
+    R_FalseValue ;
+    R_GlobalEnv ;
+    R_LevelsSymbol ;
+    R_LogicalNAValue ;
+    R_MethodsNamespace ;
+    R_MissingArg ;
+    R_ModeSymbol ;
+    R_NamespaceEnvSymbol ;
     R_NamespaceRegistry ;
     R_NamespaceSymbol ;
-    R_MethodsNamespace ;
-    R_TrueValue ;
-    R_FalseValue ;
-    R_LogicalNAValue ;
-    R_UnboundValue ;
-    R_MissingArg ;
-    R_DotsSymbol ;
+    R_NamesSymbol ;
+    R_NameSymbol  ;
+    R_NaRmSymbol ;
+    R_NilValue ;
+    R_PackageSymbol ;
+    R_PreviousSymbol ;
     R_QuoteSymbol ;
-    R_ClassSymbol ;
-    R_RowNamesSymbol ].
+    R_RecursiveSymbol ;
+    R_RowNamesSymbol ;
+    R_SeedsSymbol ;
+    R_SortListSymbol ;
+    R_SourceSymbol ;
+    R_SpecSymbol ;
+    R_SrcfileSymbol ;
+    R_SrcrefSymbol ;
+    R_TmpvalSymbol ;
+    R_TripleColonSymbol ;
+    R_TrueValue ;
+    R_TspSymbol ;
+    R_UnboundValue ;
+    R_UseNamesSymbol ;
+    R_WholeSrcrefSymbol ].
 
-(** The following property translates the [{o with f := v}] syntax from
- * OCaml as a property. Intuitively, we have
- * [globals_with g [(C1, p1);... ; (Cn, pn)] g'] if and only if
- * [g' = {g with C1 := p1, ..., Cn := pn}]. **)
-Record globals_with g (L : list ((Globals -> SExpRec_pointer) * SExpRec_pointer)) g' := {
-    globals_with_in : forall C p,
-      Mem (C, p) L ->
-      C g' = p ;
-    globals_with_out : forall C,
-      (forall p, ~ Mem (C, p) L) ->
-      Mem C Globals_constructors ->
-      C g' = C g ;
-  }.
-
-(** Solves a goal of the form [{g' | globals_with g L g'}] with an instanciated [L]. **)
-Ltac solve_globals_with :=
-  let g := fresh "g" in
-  refine (let g := make_Globals in _); repeat refine (let g := g _ in _);
-  exists g; constructors;
-  [ let M := fresh "M" in introv M;
-    repeat (inverts M as M; [ simpl; reflexivity |]); inverts M
-  | let NM := fresh "NM" in introv NM;
-    let M := fresh "M" in introv M;
-    repeat (inverts M as M; [ try solve [ simpl; reflexivity
-                                        | false NM; repeat constructors ] |]); inverts M ].
-
-(** The following tactics builds a term [g'] such that [globals_with g L g']. **)
-Ltac build_globals_with g L :=
-  let g' := fresh "g" in
-  exact (proj1_sig (ltac:(solve_globals_with) : { g' | globals_with g L g' })).
-
-Delimit Scope globals_scope with globals.
-
-(** Hidding the tactic under a readable notation. **)
-Notation "'{{!' g 'with' L '!}}'" :=
-  (ltac:(build_globals_with g L)) : globals_scope.
-
-Open Scope globals.
-
-(** A dummy element of [Globals], in which all fields are mapped to [NULL]. **)
-Definition empty_globals : Globals.
-  refine (proj1_sig (P := fun g => forall C, Mem C Globals_constructors -> C g = NULL) _).
-  refine (let g := make_Globals in _). repeat refine (let g := g _ in _). exists g.
-  introv M. repeat (inverts M as M; [simpl; reflexivity|]). inverts M.
-Defined.
-
-Lemma empty_globals_constructors : forall C,
-  Mem C Globals_constructors ->
-  C empty_globals = NULL.
-Proof.
-  introv M. repeat (inverts M as M; [ reflexivity |]). inverts M.
-Qed.
-
-(** A dummy pointer different than [NULL]. **)
-Definition dummy_not_NULL : { p : SExpRec_pointer | p <> NULL }.
-  exists (Some arbitrary : SExpRec_pointer). discriminate.
-Defined.
-
-Lemma No_duplicates_Globals_constructors : No_duplicates Globals_constructors.
-Proof.
-  repeat constructors;
-  abstract
-    (introv M; repeat (inverts M as M; [
-       match type of M with ?C1 = ?C2 =>
-         set (g := {{! empty_globals with [(C1, proj1_sig dummy_not_NULL)] !}});
-         asserts E: (C1 g = C2 g); [ rewrite M; reflexivity | inverts E ]
-       end |]);
-     inverts M).
-Qed.
-
-(** The notation [{{! g with L !}}] is useful. Unfortunately, it is actually a
- * tactic, and only works if the list [L] is known at extraction time. There
- * exists a place in the module Rinit in which the list [L] is computed at
- * execution time (its constructors are however known before, but it would make
- * the definition less readable that way). We here propose need something else
- * to deal with such list: having a computable equivalent of [{{! g with L !}}].
- * Note that as [{{! g with L !}}] is faster at execution time, it is still
- * preferable when possible. **)
-
-Definition Globals_with (g : Globals) (C : Globals -> SExpRec_pointer) (v : SExpRec_pointer) :
-    Mem C Globals_constructors ->
-    { g' | globals_with g [(C, v)] g' }.
-  introv M0. lets M: M0. lets ND: No_duplicates_Globals_constructors.
-  repeat match type of M with
-    | Mem _ [?C0] =>
-      let E := fresh "E" in
-      asserts E: (C = C0);
-      [ inverts M as M; [ reflexivity | inverts M ]
-      | clear M; rewrite E; solve_globals_with ]
-    | Mem _ ?l =>
-      let M1 := fresh "M" in
-      (forwards M1: divide_list_Mem M; [ apply surjective_pairing |]);
-      let ND1 := fresh "ND" in let ND2 := fresh "ND" in
-      (forwards (ND1&ND2): divide_list_No_duplicates ND; [ reflexivity |]);
-      let g' := fresh "g" in
-      set (g' :=
-        let L := map (fun C => (C, proj1_sig dummy_not_NULL)) (fst (divide_list l)) in
-        ltac:(solve_globals_with) : { g' | globals_with empty_globals L g' });
-      let E := fresh "E" in
-      destruct (C (proj1_sig g')) eqn: E;
-      [ (* [Some] case: we are in the first list. *)
-        asserts M': (Mem C (fst (divide_list l)));
-        [ inverts M1 as M1;
-          [ eassumption
-          | erewrite globals_with_out in E;
-            [ rewrite empty_globals_constructors in E; [ inverts E | apply M0 ]
-            | apply (proj2_sig g')
-            | let MA := fresh "M" in let M2 := fresh "M" in let E' := fresh "E" in
-              introv MA; forwards (?&M2&E'): Mem_map_inv (rm MA); inverts E';
-              applys divide_list_Mem_No_duplicates M ND M2 M1; reflexivity
-            | apply M0 ]
-        ]
-        | clear ND ND2 M; rename M' into M; rename ND1 into ND ]
-      | (* [None] case: we are in the second list. *)
-        asserts M': (Mem C (snd (divide_list l))) ;
-        [ inverts M1 as M1;
-          [ erewrite globals_with_in with (p := proj1_sig dummy_not_NULL) in E;
-            [ inverts E
-            | apply (proj2_sig g')
-            | apply Mem_map with (f := fun C => (C, proj1_sig dummy_not_NULL)); apply M1 ]
-          | eassumption ]
-        | clear ND ND1 M; rename M' into M; rename ND2 into ND ]
-      ];
-      clear M1 E g'; simpl in M
-  end.
-Defined.
-
-Lemma Globals_constructors_all : forall g g',
-  (forall C, Mem C Globals_constructors -> C g = C g') ->
+(** No projection is missing in [Globals_projections]. **)
+Lemma Globals_projections_all : forall g g',
+  (forall C, Mem C Globals_projections -> C g = C g') ->
   g = g'.
 Proof.
   introv F. destruct g, g'.
@@ -203,15 +165,30 @@ Proof.
       | simpl in E; rewrite E; clear E ];
       t l'
     end in
-  let l := eval unfold Globals_constructors in Globals_constructors in
+  let l := eval unfold Globals_projections in Globals_projections in
   t l.
 Qed.
+
+
+(** The following property translates the [{o with f := v}] syntax from
+ * OCaml as a property. Intuitively, we have
+ * [globals_with g [(C1, p1);... ; (Cn, pn)] g'] if and only if
+ * [g' = {g with C1 := p1, ..., Cn := pn}]. **)
+Record globals_with g (L : list ((Globals -> SExpRec_pointer) * SExpRec_pointer)) g' := {
+    globals_with_in : forall C p,
+      Mem (C, p) L ->
+      C g' = p ;
+    globals_with_out : forall C,
+      (forall p, ~ Mem (C, p) L) ->
+      Mem C Globals_projections ->
+      C g' = C g ;
+  }.
 
 Lemma globals_with_empty : forall g g',
   globals_with g nil g' <-> g = g'.
 Proof.
   iff G.
-  - apply Globals_constructors_all. introv M.
+  - apply Globals_projections_all. introv M.
     symmetry. applys~ globals_with_out G. introv M'. inverts M'.
   - constructors.
     + introv M. inverts M.
@@ -220,7 +197,7 @@ Qed.
 
 Lemma globals_with_transitive : forall g1 g2 g3 L1 L2 L1',
   globals_with g1 L1 g2 ->
-  (forall C v, Mem (C, v) L1 -> Mem C Globals_constructors) ->
+  (forall C v, Mem (C, v) L1 -> Mem C Globals_projections) ->
   globals_with g2 L2 g3 ->
   Filter (fun C_v => ~ exists v, Mem (fst C_v, v) L2) L1 = L1' ->
   globals_with g1 (L1' ++ L2) g3.
@@ -254,7 +231,7 @@ Qed.
 
 Lemma globals_with_transitive_step : forall g1 g2 g3 C1 v1 L2,
   globals_with g1 [(C1, v1)] g2 ->
-  Mem C1 Globals_constructors ->
+  Mem C1 Globals_projections ->
   (forall v, ~ Mem (C1, v) L2) ->
   globals_with g2 L2 g3 ->
   globals_with g1 ((C1, v1) :: L2) g3.
@@ -268,22 +245,144 @@ Proof.
     + lets (v&MI): (rm I). false* F.
 Qed.
 
+
+(** Solves a goal of the form [{g' | globals_with g L g'}] with an instanciated [L]. **)
+Ltac solve_globals_with :=
+  let g := fresh "g" in
+  refine (let g := make_Globals in _); repeat refine (let g := g _ in _);
+  exists g; constructors;
+  [ let M := fresh "M" in introv M;
+    repeat (inverts M as M; [ simpl; reflexivity |]); inverts M
+  | let NM := fresh "NM" in introv NM;
+    let M := fresh "M" in introv M;
+    repeat (inverts M as M; [ try solve [ simpl; reflexivity
+                                        | false NM; repeat constructors ] |]); inverts M ].
+
+(** The following tactics builds a term [g'] such that [globals_with g L g']. **)
+Ltac build_globals_with g L :=
+  let g' := fresh "g" in
+  exact (proj1_sig (ltac:(solve_globals_with) : { g' | globals_with g L g' })).
+
+Delimit Scope globals_scope with globals.
+
+(** Hidding the tactic under a readable notation. **)
+Notation "'{{!' g 'with' L '!}}'" :=
+  (ltac:(build_globals_with g L)) : globals_scope.
+
+Open Scope globals.
+
+(** A dummy element of [Globals], in which all fields are mapped to [NULL]. **)
+Definition empty_globals : Globals.
+  refine (proj1_sig (P := fun g => forall C, Mem C Globals_projections -> C g = NULL) _).
+  refine (let g := make_Globals in _). repeat refine (let g := g _ in _). exists g.
+  introv M. repeat (inverts M as M; [simpl; reflexivity|]). inverts M.
+Defined.
+
+Lemma empty_globals_projections : forall C,
+  Mem C Globals_projections ->
+  C empty_globals = NULL.
+Proof.
+  introv M. repeat (inverts M as M; [ reflexivity |]). inverts M.
+Qed.
+
+(** Solves a goal of the form [No_duplicates L], where [L] is a list
+ * of projections of [Globals]. **)
+Ltac prove_no_duplicate_projections :=
+  let M := fresh "M" in let E := fresh "E" in
+  repeat (apply No_duplicates_cons;
+    [ abstract
+        (introv M; repeat (inverts M as M; [
+           match type of M with ?C1 = ?C2 =>
+             set (g := {{! empty_globals with [(C1, proj1_sig dummy_not_NULL)] !}});
+             asserts E: (C1 g = C2 g); [ rewrite M; reflexivity | inverts E ]
+           end |]);
+         inverts M)
+    |]); apply No_duplicates_nil.
+
+(** No projection appears twice in [Globals_projections]. **)
+Lemma No_duplicates_Globals_projections : No_duplicates Globals_projections.
+Proof.
+  prove_no_duplicate_projections.
+Qed.
+
+
+(** The notation [{{! g with L !}}] is useful. Unfortunately, it is actually a
+ * tactic, and only works if the list [L] is known at extraction time. There
+ * exists a place in the module Rinit in which the list [L] is computed at
+ * execution time (its projections are however known before, but it would make
+ * the definition less readable that way). We here propose need something else
+ * to deal with such list: having a computable equivalent of [{{! g with L !}}].
+ * Note that as [{{! g with L !}}] is faster at execution time, it is still
+ * preferable when possible. **)
+
+Definition Globals_with (g : Globals) (C : Globals -> SExpRec_pointer) (v : SExpRec_pointer) :
+    Mem C Globals_projections ->
+    { g' | globals_with g [(C, v)] g' }.
+  introv M0. lets M: M0. lets ND: No_duplicates_Globals_projections.
+  repeat match type of M with
+    | Mem _ [?C0] =>
+      let E := fresh "E" in
+      asserts E: (C = C0);
+      [ inverts M as M; [ reflexivity | inverts M ]
+      | clear M; rewrite E; solve_globals_with ]
+    | Mem _ ?l =>
+      let M1 := fresh "M" in
+      (forwards M1: divide_list_Mem M; [ apply surjective_pairing |]);
+      let ND1 := fresh "ND" in let ND2 := fresh "ND" in
+      (forwards (ND1&ND2): divide_list_No_duplicates ND; [ reflexivity |]);
+      let g' := fresh "g" in
+      set (g' :=
+        let L := map (fun C => (C, proj1_sig dummy_not_NULL)) (fst (divide_list l)) in
+        ltac:(solve_globals_with) : { g' | globals_with empty_globals L g' });
+      let E := fresh "E" in
+      destruct (decide (C (proj1_sig g') = NULL)) eqn: E; fold_bool; rew_refl in E;
+      [ (* [true] case: we are in the second list. *)
+        asserts M': (Mem C (snd (divide_list l)));
+        [ inverts M1 as M1;
+          [ erewrite globals_with_in with (p := proj1_sig dummy_not_NULL) in E;
+            [ false~ (proj2_sig dummy_not_NULL)
+            | apply (proj2_sig g')
+            | apply Mem_map with (f := fun C => (C, proj1_sig dummy_not_NULL)); apply M1 ]
+          | eassumption ]
+        | clear ND ND1 M; rename M' into M; rename ND2 into ND ]
+      | (* [false] case: we are in the first list. *)
+        asserts M': (Mem C (fst (divide_list l)));
+        [ inverts M1 as M1;
+          [ eassumption
+          | erewrite globals_with_out in E;
+            [ rewrite empty_globals_projections in E; [ false~ E | apply M0 ]
+            | apply (proj2_sig g')
+            | let MA := fresh "M" in let M2 := fresh "M" in let E' := fresh "E" in
+              introv MA; forwards (?&M2&E'): Mem_map_inv (rm MA); inverts E';
+              applys divide_list_Mem_No_duplicates M ND M2 M1; reflexivity
+            | apply M0 ]
+        ]
+        | clear ND ND2 M; rename M' into M; rename ND1 into ND ]
+      ];
+      clear M1 E g'; simpl in M
+  end.
+Defined.
+
 Definition Globals_with_list (g : Globals) (L : list ((Globals -> SExpRec_pointer) * SExpRec_pointer)) :
-    (forall C v, Mem (C, v) L -> Mem C Globals_constructors) ->
+    (forall C v, Mem (C, v) L -> Mem C Globals_projections) ->
     No_duplicates (map fst L) ->
     { g' | globals_with g L g' }.
   introv F ND. gen g. induction L; introv.
   - exists g. rewrite~ globals_with_empty.
-  - destruct a as [C v]. asserts M: (Mem C Globals_constructors).
+  - destruct a as [C v]. asserts M: (Mem C Globals_projections).
     + apply~ F.
     + forwards IHg: IHL (proj1_sig (Globals_with g C v M)).
       * introv M'. apply~ F. apply* Mem_next.
       * inverts~ ND.
-      * exists (proj1_sig (Globals_with (proj1_sig IHg) C v M)).
-        apply~ globals_with_transitive_step.
-        -- refine (proj2_sig (Globals_with _ _ _ _)). apply~ F.
+      * exists (proj1_sig IHg). apply~ globals_with_transitive_step.
+        -- refine (proj2_sig (Globals_with _ _ _ M)).
         -- introv M'. rew_list in ND. inverts ND as NM ND. false NM.
            applys Mem_map M'.
-        -- refine (proj2_sig (Globals_with _ _ _ _)).
+        -- apply~ proj2_sig.
 Defined.
+
+(** We can now prove a notation for this function. **)
+Notation "'{{' g 'with' L 'using' F ',' ND '}}'" :=
+  (Globals_with_list g L F ND) : globals_scope.
+
 
